OCLtoSQL.thy
@@ -94,11 +94,16 @@ fun collectAux :: "val list \<Rightarrow> OCLexp \<Rightarrow> Enrollment \<Righ
 
 COMMENT *)
 
+fun getAssignedPerson :: "string \<Rightarrow> Person list \<Rightarrow> Person" where
+"getAssignedPerson s [] = Person.PNULL"
+| "getAssignedPerson s (p#ps) = (if (s = (getIdPerson p)) then p else (getAssignedPerson s ps))"
+
+
 fun eval :: "OCLexp \<Rightarrow> Objectmodel \<Rightarrow> val list" where
 "eval (MyOCL.Int i) om = [VInt i]"
 | "eval (MyOCL.Var x) om = [VObj x]"
 | "eval (MyOCL.Eq e1 e2) om = [VBool (equalValList (eval e1 om) (eval e2 om))]" 
-| "eval (MyOCL.Att (Var v) att) om = [(projValAtt att (VPerson (PVObj v)))]"
+| "eval (MyOCL.Att (Var v) att) om = [(projValAtt att (VPerson (getAssignedPerson v (getPersonList om))))]"
 | "eval (MyOCL.As (Var v) as) om = projValAs as (VObj v) (getEnrollmentList om)"
 
 (* COMMENT
